examples/knot/Knot01proof.v
@@ -85,8 +85,9 @@ End AUX.
 Section SIMMODSEM.
 
   Context `{Σ: GRA.t}.
-  Context `{@GRA.inG knotRA Σ}.
+  Context `{@GRA.inG invRA Σ}.
   Context `{@GRA.inG memRA Σ}.
+  Context `{@GRA.inG knotRA Σ}.
 
   Let W: Type := (Σ * Any.t) * (Σ * Any.t).
 
@@ -96,29 +97,20 @@ Section SIMMODSEM.
 
   Let wf (skenv: SkEnv.t): W -> Prop :=
     fun '(mrps_src0, mrps_tgt0) =>
-      exists (mr: Σ)(f': option (nat -> nat)),
+      exists (mr: Σ),
         (<<SRC: mrps_src0 = (mr, tt↑)>>) /\
         (<<TGT: mrps_tgt0 = (ε, tt↑)>>) /\
-        (<<SEP: iHyp ((Own (GRA.embed (knot_frag f')))
-                      ∨
-                      ((Own (GRA.embed (knot_full f')))
-                         **
-                         (Exists fb',
-                          (Own (knot_var skenv fb'))
-                            **
-                            (⌜forall f (EQ: f' = Some f),
-                                  exists fb fn,
-                                    (<<BLK: fb' = Vptr fb 0>>) /\
-                                    (<<FN: skenv.(SkEnv.blk2id) fb = Some fn>>) /\
-                                    (<<FIND: List.find (fun '(_fn, _) => dec fn _fn) (FunStb skenv) = Some (fn, fun_gen RecStb skenv f)>>)⌝)))) mr>>).
-
-        (<<TGT: mrps_tgt0 = (ε, fb'↑)>>) /\
-        (<<SIM: (iHyp (Own (GRA.embed (knot_full f'))) mr)>>) /\
-        (<<SOME: forall f (FUN: f' = Some f),
-            exists fb,
-              (<<BLK: fb' = Some fb>>) /\
-              (<<FN: fb_has_spec skenv (FunStb skenv) fb (fun_gen RecStb skenv f)>>)>>)
-  .
+        (<<SEP: (inv_closed
+                 ∨
+                 ((inv_open)
+                    **
+                    (Exists (f': option (nat -> nat)) (fb': val),
+                     (⌜forall f (EQ: f' = Some f),
+                           exists fb,
+                             (<<BLK: fb' = Vptr fb 0>>) /\
+                             (<<FN: fb_has_spec skenv (FunStb skenv) fb (fun_gen RecStb skenv f)>>)⌝)
+                       ** (Own (GRA.embed (knot_full f')))
+                       ** (Own (knot_var skenv fb'))))) mr>>).
 
   Hypothesis RecStb_incl: forall skenv,
       stb_incl KnotRecStb (RecStb skenv).
@@ -126,14 +118,8 @@ Section SIMMODSEM.
   Hypothesis FunStb_incl: forall skenv,
       stb_incl (FunStb skenv) (GlobalStb skenv).
 
-  Variable MemStb_incl
-    :
-      forall skenv fn fsp
-             (SPECS: List.find (fun '(_fn, _) => dec fn _fn) MemStb = Some fsp),
-        List.find (fun '(_fn, _) => dec fn _fn) (GlobalStb skenv) = Some fsp.
-
-  (* AUX END -------------------------------------------- *)
-
+  Variable MemStb_incl: forall skenv,
+      stb_incl MemStb (GlobalStb skenv).
 
   Theorem correct: ModPair.sim (Knot1.Knot RecStb FunStb GlobalStb) Knot0.Knot.
   Proof.
@@ -141,75 +127,125 @@ Section SIMMODSEM.
     i. eapply adequacy_lift.
     econstructor 1 with (wf:=wf (Sk.load_skenv sk)); et; ss.
     2: {
-      eexists. exists None. esplits; ss. right.
+      eexists. esplits; ss. right.
+      exists (GRA.embed inv_black), (knot_var sk Vundef ⋅ GRA.embed (knot_full None)).
+      splits; ss.
+      { r_solve. }
+      { exists ε. r_solve. }
+      exists None, Vundef.
       exists (GRA.embed (knot_full None)), (knot_var sk Vundef). splits; ss.
-      { apply URA.add_comm. }
-      { exists ε. rewrite URA.unit_id. ss. }
-      { exists Vundef. exists (knot_var sk Vundef), (@URA.unit Σ). splits; ss.
-        { rewrite URA.unit_id. ss. }
-        { exists ε. rewrite URA.unit_id. ss. }
-      }
+      { r_solve. }
+      2: { exists ε. r_solve. }
+      exists ε, (GRA.embed (knot_full None)). splits; ss.
+      { r_solve. }
+      { exists ε. r_solve. }
     }
     hexploit (SKINCL "rec"); ss; eauto. intros [blk0 FIND0].
     hexploit (SKINCL "_f"); ss; eauto. intros [blk1 FIND1].
     econs; ss; [|econs; ss].
     { init. unfold recF, ccall. harg_tac. iRefresh.
       destruct x as [f n]. ss. des. subst.
-      iRefresh. iDestruct PRE. iPure A. des; clarify.
-      eapply Any.upcast_inj in A. des; clarify. steps.
-      rewrite Any.upcast_downcast in _UNWRAPN. clarify. astart 1.
-      assert (f' = Some f); subst.
-      { hexploit knot_ra_merge; et. intro T. iSpecialize T SIM. iSpecialize T PRE. iPure T. auto. }
-      hexploit SOME; eauto. clear SOME. i. des. clarify. steps.
-      rewrite Any.upcast_downcast. ss. steps.
-      dup FN. inv FN. rewrite FBLOCK. steps.
-      hexploit (SKINCL "rec"); ss; eauto. i. des. rewrite H0. ss. steps.
-      inv SPEC. exploit FunStb_incl; et. i.
+      iRefresh. iDestruct PRE. iDestruct PRE. iPure PRE. des; clarify.
+      eapply Any.upcast_inj in PRE. des; clarify. steps.
+      rewrite Any.upcast_downcast in _UNWRAPN. clarify. astart 2.
+      iDestruct SEP.
+      { inv_clear. }
+      iDestruct SEP. iDestruct A1. iDestruct A1. iDestruct A1. iDestruct A1. iPure A1.
+      iExploitP (@knot_ra_merge _ _ x4 (Some f)). i. subst.
+      hexploit A1; eauto. clear A1. i. des. clarify. steps.
+      rewrite FIND1. steps.
       acatch.
-      { eapply x1. }
-      hcall_tac_weaken (fun_gen RecStb skenv f) n (ord_pure (2 * n)) SIM (@URA.unit Σ) PRE.
-      { et. }
-      { ss. splits; ss. iRefresh. iSplitR PRE; ss.
-        red. red. esplits; eauto. econs; eauto.
+      { eapply MemStb_incl. stb_tac. ss. }
+      iMerge A3 A0. iMerge A3 SEP.
+      hcall_tac (blk1, 0%Z, Vptr fb 0) (ord_pure 0) A A3 A2.
+      { ss. splits; ss. iRefresh. iSplitL A2; ss. iSplitR A2; ss.
+        unfold knot_var in *. rewrite FIND1 in *. ss. }
+      { splits; ss. eauto with ord_step. }
+      { red. eexists. esplits; eauto. left. ss. }
+      steps. des. iRefresh. iDestruct POST. iPure A.
+      rewrite Any.upcast_downcast in _UNWRAPN. clarify.
+      eapply Any.upcast_inj in A. des; clarify. steps.
+      dup FN. inv FN. inv SPEC. rewrite FBLOCK. steps.
+      rewrite FIND0. steps. acatch.
+      { eapply FunStb_incl. eapply FIND. }
+      iDestruct A3. iDestruct A3. iDestruct SEP.
+      2:{ iDestruct SEP. inv_clear. }
+      iMerge A0 SEP. iMerge A POST. iMerge A A3.
+      hcall_tac_weaken (fun_gen RecStb sk f) n (ord_pure (2 * n)) A (@URA.unit Σ) A0; ss.
+      { split; auto. iRefresh. iDestruct A0. iSplitR A; ss. iSplitR A0; ss.
+        red. red. esplits; eauto. econs.
         { eapply SKWF. eauto. }
         econs.
         { eapply RecStb_incl. des_ifs. }
         { refl. }
       }
       { splits; ss. eauto with ord_step. }
-      { ss. esplits; eauto. i. clarify. esplits; eauto. }
-      des. clarify. iRefresh. iDestruct POST. iPure POST.
-      eapply Any.upcast_inj in POST. des; clarify.
-      steps. rewrite Any.upcast_downcast in _UNWRAPN. clarify.
+      { esplits; eauto. iRight.
+        iDestruct A. iDestruct A. iSplitL A; ss.
+        iExists (Some f). iExists __. iSplitR A1.
+        { iSplitR A0; ss.
+          red. red. i. clarify. esplits; eauto. }
+        { unfold knot_var. rewrite FIND1. iApply A1. }
+      }
+      steps. des. clarify. iRefresh.
+      iDestruct POST. iDestruct POST. iPure POST.
+      rewrite Any.upcast_downcast in _UNWRAPN. clarify.
+      eapply Any.upcast_inj in POST. des; clarify. iMerge A0 A.
       astop. force_l. eexists.
-      hret_tac SEP A0; ss.
-      { split; ss. iRefresh. iSplitL A0; ss. }
-      { esplits; eauto. }
+      hret_tac SEP A0.
+      { split; ss. iRefresh. iDestruct A0. iSplitR A; ss. iSplitR A0; ss. }
+      { red. esplits; eauto. }
     }
     { init. unfold knotF, ccall. harg_tac.
       ss. des. subst.
-      iRefresh. iDestruct PRE. iPure PRE. des; clarify.
-      iDestruct A. eapply Any.upcast_inj in PRE. des; clarify. steps.
-      rewrite Any.upcast_downcast in _UNWRAPN. clarify. iDestruct SEP.
-      { iExploitP (@knot_frag_unique _ _ f' x2); ss. }
-      iDestruct SEP. astart 1.
-      iMerge SEP A. rewrite <- own_sep in SEP.
-      eapply own_upd in SEP; cycle 1; [|rewrite intro_iHyp in SEP;iUpdate SEP].
+      iRefresh. iDestruct PRE. iDestruct PRE. iPure PRE. des; clarify.
+      eapply Any.upcast_inj in PRE. des; clarify.
+      iDestruct A0. iDestruct SEP.
+      { inv_clear. }
+      rewrite Any.upcast_downcast. steps.
+      iDestruct SEP. iDestruct A1. iDestruct A1.
+      iDestruct A1. iDestruct A1.
+      unfold knot_var in *. rewrite FIND1 in *. steps.
+      astart 1. acatch.
+      { eapply MemStb_incl. stb_tac. ss. }
+      iMerge A3 A0. iMerge A3 SEP.
+      hcall_tac (blk1, 0%Z, Vptr fb 0) (ord_pure 0) A A3 A2.
+      { ss. splits; ss. iRefresh. iExists __. iSplitL A2; ss.
+        iSplitR A2; ss. iApply A2. }
+      { splits; ss. eauto with ord_step. }
+      { red. esplits; eauto. left. ss. }
+      steps. astop. des; clarify.
+      rewrite Any.upcast_downcast in _UNWRAPN. clarify.
+      iDestruct A3. iDestruct A3. iDestruct SEP.
+      2: { iDestruct SEP. inv_clear. }
+      iExploitP (@knot_ra_merge _ _ x6 x0). i. subst.
+      iMerge A3 A0. rewrite <- own_sep in A3.
+      eapply own_upd in A3; cycle 1; [|rewrite intro_iHyp in A3;iUpdate A3].
       { rewrite GRA.embed_add. eapply GRA.embed_updatable.
         instantiate (1:= knot_full (Some x) ⋅ knot_frag (Some x)).
-        eapply Auth.auth_update. rr. ii. des; ss. ur in FRAME. ur. destruct ctx; ss; clarify.
+        eapply Auth.auth_update. rr. ii. des; ss.
+        ur in FRAME. ur. destruct ctx; ss; clarify.
       }
-      rewrite <- GRA.embed_add in SIM. rewrite own_sep in SIM. iDestruct SIM.
+      replace tmp0 with (x12 ⋅ x13); [|admit "iMerge bug"].
+      rewrite <- GRA.embed_add in A3. rewrite own_sep in A3. iDestruct A3.
+      steps. rewrite FIND0. steps.
+      iMerge POST A. iMerge POST A3. iMerge SEP A0.
       force_l. eexists.
-      hret_tac SIM A; ss.
-      { esplits; eauto. iRefresh. iSplitR A; eauto. red. red. esplits; eauto.
-        econs; eauto.
-        { eapply SKWF; eauto. }
-        econs.
-        { eapply RecStb_incl; eauto. ss. }
-        { refl. }
+      hret_tac POST SEP.
+      { split; eauto. iRefresh. iDestruct SEP. iSplitR SEP; ss.
+        iSplitR A; ss.
+        { red. red. esplits; eauto. econs.
+          { eapply SKWF. eauto. }
+          econs.
+          { eapply RecStb_incl. ss. }
+          { refl. }
+        }
       }
-      { esplits; eauto. i. clarify. esplits; eauto. }
+      { red. esplits; eauto. iRight. iDestruct POST. iDestruct POST.
+        iSplitL A0; ss. iExists (Some x). iExists __. iSplitR POST.
+        { iSplitR A; ss. red. red. i. clarify. esplits; eauto. }
+        { rewrite Heq. ss. }
+      }
     }
   Qed.
 
